\documentclass[12pt]{article}
 
\usepackage[margin=1in]{geometry} 
\usepackage{amsmath,amsthm,amssymb}
\usepackage{bm} % for bold math symbols
\usepackage{amstext} % for \text macro
\usepackage{array}   % for \newcolumntype macro
\newcolumntype{L}{>{$}l<{$}} % math-mode version of "l" column type
\newcolumntype{C}{>{$}c<{$}} % math-mode version of "c" column type
\newcolumntype{R}{>{$}r<{$}} % math-mode version of "r" column type
 
\newcommand{\N}{\mathbb{N}}
\newcommand{\Z}{\mathbb{Z}}

\newenvironment{theorem}[2][Theorem]{\begin{trivlist}
\item[\hskip \labelsep {\bfseries #1}\hskip \labelsep {\bfseries #2.}]}{\end{trivlist}}
\newenvironment{lemma}[2][Lemma]{\begin{trivlist}
\item[\hskip \labelsep {\bfseries #1}\hskip \labelsep {\bfseries #2.}]}{\end{trivlist}}
\newenvironment{exercise}[2][Exercise]{\begin{trivlist}
\item[\hskip \labelsep {\bfseries #1}\hskip \labelsep {\bfseries #2.}]}{\end{trivlist}}
\newenvironment{reflection}[2][Reflection]{\begin{trivlist}
\item[\hskip \labelsep {\bfseries #1}\hskip \labelsep {\bfseries #2.}]}{\end{trivlist}}
\newenvironment{proposition}[2][Proposition]{\begin{trivlist}
\item[\hskip \labelsep {\bfseries #1}\hskip \labelsep {\bfseries #2.}]}{\end{trivlist}}
\newenvironment{corollary}[2][Corollary]{\begin{trivlist}
\item[\hskip \labelsep {\bfseries #1}\hskip \labelsep {\bfseries #2.}]}{\end{trivlist}}

\begin{document}



\noindent
\large\textbf{HW 6, Problem 03} \hfill \textbf{Gregory Linkowski} \\
\normalsize CS 450 / ECE 491 \hfill linkows2 \\
Michael Heath \hfill due 11/14/16 \\


\vspace{5mm}
Write each of the following ODEs as an equivalent first-order system of ODEs:
\vspace{-2mm} \\

\begin{exercise}{1}
	Van der Pol eq: $\quad y'' = y'(1-y^2) - y$
\end{exercise} \vspace{-10mm}
\begin{proof}[]
	\begin{align*}
		\begin{cases} x_1 = y \\ x_2 = y' \end{cases}
		& \Rightarrow \begin{cases}
			\dot{x_1} = x_2 \\
			\dot{x_2} = x_2 - x_2 x_1^2 - x_1
		\end{cases}
	\end{align*}
	\textbf{Answer 1.} \vspace{-7mm} \\
		\[ \boxed{  } \]
\end{proof}

\begin{exercise}{2}
	Blasius eq: $\quad y'''  = -y y''$
\end{exercise} \vspace{-10mm}
\begin{proof}[]
	\begin{align*}
	\begin{cases} x_1 = y \\ x_2 = y' \\ x_3 = y'' \end{cases}
	& \Rightarrow \begin{cases}
	\dot{x_1} = x_2 \\
	\dot{x_2} = x_3 \\
	\dot{x_3} = - x_1 x_3
	\end{cases}
	\end{align*}
	\textbf{Answer 2.} \vspace{-7mm} \\
	\[ \boxed{  } \]
\end{proof}

\begin{exercise}{3}
	Newton's Second Law of Motion for two-body problem:
	\[ 	y_1'' = \frac{- G M y_1}{(y_1^2 + y_2^2)^\frac{3}{2}} \quad
		y_2'' = \frac{- G M y_2}{(y_1^2 + y_2^2)^\frac{3}{2}} \] 
\end{exercise} \vspace{-10mm}
\begin{proof}[]
	\begin{align*}
	\begin{cases} x_1 = y_1 \\ x_2 = y_1' \\ x_3 = y_3 \\ x_4 = y_3' \end{cases}
	& \Rightarrow \begin{cases}
	\dot{x_1} = x_2 \\
	\dot{x_2} = - G M x_1 / (x_1^2 + x_3^2)^\frac{3}{2} \\
	\dot{x_3} = x_4 \\
	\dot{x_4} = - G M x_3 / (x_1^2 + x_3^2)^\frac{3}{2}
	\end{cases}
	\end{align*}
	\textbf{Answer 3.} \vspace{-7mm} \\
	\[ \boxed{  } \]
\end{proof}


\end{document}