\documentclass[12pt]{article}
 
\usepackage[margin=1in]{geometry} 
\usepackage{amsmath,amsthm,amssymb}
\usepackage{bm} % for bold math symbols
\usepackage{amstext} % for \text macro
\usepackage{array}   % for \newcolumntype macro
\newcolumntype{L}{>{$}l<{$}} % math-mode version of "l" column type
\newcolumntype{C}{>{$}c<{$}} % math-mode version of "c" column type
\newcolumntype{R}{>{$}r<{$}} % math-mode version of "r" column type
 
\newcommand{\N}{\mathbb{N}}
\newcommand{\Z}{\mathbb{Z}}

\newenvironment{theorem}[2][Theorem]{\begin{trivlist}
\item[\hskip \labelsep {\bfseries #1}\hskip \labelsep {\bfseries #2.}]}{\end{trivlist}}
\newenvironment{lemma}[2][Lemma]{\begin{trivlist}
\item[\hskip \labelsep {\bfseries #1}\hskip \labelsep {\bfseries #2.}]}{\end{trivlist}}
\newenvironment{exercise}[2][Exercise]{\begin{trivlist}
\item[\hskip \labelsep {\bfseries #1}\hskip \labelsep {\bfseries #2.}]}{\end{trivlist}}
\newenvironment{reflection}[2][Reflection]{\begin{trivlist}
\item[\hskip \labelsep {\bfseries #1}\hskip \labelsep {\bfseries #2.}]}{\end{trivlist}}
\newenvironment{proposition}[2][Proposition]{\begin{trivlist}
\item[\hskip \labelsep {\bfseries #1}\hskip \labelsep {\bfseries #2.}]}{\end{trivlist}}
\newenvironment{corollary}[2][Corollary]{\begin{trivlist}
\item[\hskip \labelsep {\bfseries #1}\hskip \labelsep {\bfseries #2.}]}{\end{trivlist}}

\begin{document}



\noindent
\large\textbf{HW 3, Problem 04} \hfill \textbf{Gregory Linkowski} \\
\normalsize CS 450 / ECE 491 \hfill linkows2 \\
Michael Heath \hfill due 10/5/16 \\



\vspace{5mm}
Let	$ f(x) - x^2 - 3x + 2 = 0 $.
Analyze the following fixed-point problems for $x=2$ by considering $|g_i'(2)|$.
\vspace{5mm}

\begin{exercise}{1} $g_1(x) = \frac{x^2 + 2}{3}$
\end{exercise}
\begin{proof}[]
	\vspace{-8mm}
	\begin{align*}
		g_1'(x) &= \frac{d}{dx}\left[  \frac{1}{3}x^2 + \frac{2}{3} \right] \\
		 &= \frac{2}{3}x
	\end{align*}
	\[\boxed{ \; |g_1'(2)| = \frac{4}{3} > 1 \; }\]
	\quote{Fixed-point iteration is expected to be \underline{divergent}.}
\end{proof}

\begin{exercise}{2} $g_2(x) = \sqrt{3x - 2}$
\end{exercise}
\begin{proof}[]
	\vspace{-8mm}
	\begin{align*}
		g_2'(x) &= \frac{d}{dx}\left[  (3x - 2)^{\frac{1}{2}} \right] \\
		&= \frac{1}{2} \times 3 (3x - 2)^{-\frac{1}{2}} \\
		&= \frac{3}{2 \sqrt{3x - 2}}
	\end{align*}
	\[\boxed{ \; |g_2'(2)| = \frac{3}{4} < 1 \; }\] 
	\quote{Fixed-point iteration is expected to be \underline{linearly convergent}.}
\end{proof}

\begin{exercise}{3} $g_3(x) = 3 - \frac{2}{x}$
\end{exercise}
\begin{proof}[]
	\vspace{-8mm}
	\begin{align*}
		g_3'(x) &= \frac{d}{dx}\left[  3 - 2x^{-1} \right] \\
		&= 2x^{-2} \\
		&= \frac{2}{x^2}
	\end{align*}
	\[\boxed{ \; |g_3'(2)| = \frac{1}{2} < 1 \; }\] 
	\quote{Fixed-point iteration is expected to be \underline{linearly convergent}.}
\end{proof}

\begin{exercise}{4} $g_4(x) = \frac{x^2 - 2}{2x - 3}$
\end{exercise}
\begin{proof}[]
	\vspace{-8mm}
	\begin{align*}
		g_2'(x) &= \frac{d}{dx}\left[  (x^2 - 2)(2x - 3)^{-1} \right] \\
		&= 2x(2x - 3)^{-1} + (x^2 - 2)(-1)2(2x-3)^{-2} \\
		&= \frac{2x(2x-3)}{(2x - 3)^2} + \frac{-2(x^2 - 2)}{(2x-3)^2} \\
		&= \frac{4x^2 - 6x - 2x^2 + 4}{(2x-3)^2} \\
		&= \frac{2(x^2 - 3x + 2)}{(2x-3)^2} \\
	\end{align*}
	\[\boxed{ \; |g_4'(2)| = 0 < 1 \; }\] 
	\quote{Fixed-point iteration is expected to be \underline{quadratically convergent}.}
\end{proof}



\end{document}